prove duality theorems (#769)

equational_theories/Preorder.lean
@@ -6,7 +6,7 @@ open Law
 
 namespace Law.MagmaLaw
 
-variable {α : Type*}
+variable {α β : Type*}
 
 /--
 A magma law `l₁` implies a law `l₂` if in any Magma `G` where `l₁` holds, `l₂` also holds.
@@ -14,8 +14,20 @@ A magma law `l₁` implies a law `l₂` if in any Magma `G` where `l₁` holds, 
 We have to explicitly quantify the type `G` and the Magma instance `[Magma G]` instead of
 using them as parameters so that the implication holds in any Magma `G`.
 -/
-def implies (l₁ l₂ : MagmaLaw α) := ∀ {G : Type} [Magma G],
+def implies (l₁ : MagmaLaw α) (l₂ : MagmaLaw β) := ∀ {{G : Type}} [Magma G],
   satisfies G l₁ → satisfies G l₂
+
+protected def iff (l₁ : MagmaLaw α) (l₂ : MagmaLaw β) := ∀ (G : Type) [Magma G],
+  satisfies G l₁ ↔ satisfies G l₂
+
+theorem iff.symm {l₁ : MagmaLaw α} {l₂ : MagmaLaw β} (h : l₁.iff l₂) :
+    l₂.iff l₁ := fun G => (h G).symm
+
+theorem iff.mp {l₁ : MagmaLaw α} {l₂ : MagmaLaw β} (h : l₁.iff l₂) :
+    l₁.implies l₂ := fun G => (h G).1
+
+theorem iff.mpr {l₁ : MagmaLaw α} {l₂ : MagmaLaw β} (h : l₁.iff l₂) :
+    l₂.implies l₁ := h.symm.mp
 
 /--
 If a law `l₁` implies a law `l₂`, then we say `l₁ ≤ l₂`.
@@ -23,7 +35,7 @@ If a law `l₁` implies a law `l₂`, then we say `l₁ ≤ l₂`.
 instance : LE (MagmaLaw α) where
   le l₁ l₂ := l₁.implies l₂
 
-theorem implies_set {α} (l₁ l₂ : MagmaLaw α) (h : l₁.implies l₂) :
+theorem implies_set {α} {l₁ : MagmaLaw α} {l₂ : MagmaLaw β} (h : l₁.implies l₂) :
     ({ ⟨G, _⟩ | G ⊧ l₁ } : Set (Σ G : Type, Magma G)) ⊆ { ⟨G, _⟩ | G ⊧ l₂ } :=
   fun ⟨_, _⟩ h1 ↦ h h1
 
@@ -32,14 +44,14 @@ A stronger law is smaller than a weaker law, because this corresponds to the inc
 the class of magmas that obey these laws:  the class of magmas that obey the stronger law is a
 subset of the class of magmas that obey the weaker law.
 -/
-theorem le_set {α} (l₁ l₂ : MagmaLaw α) (h : l₁ ≤ l₂) :
+theorem le_set {α} {l₁ l₂ : MagmaLaw α} (h : l₁ ≤ l₂) :
     ({ ⟨G, _⟩ | G ⊧ l₁ } : Set (Σ G : Type, Magma G)) ⊆ { ⟨G, _⟩ | G ⊧ l₂ } :=
-  implies_set _ _ h
+  implies_set h
 
 /--
 The law `0 ≃ 0` is the maximal element in the pre-order on magma laws (over ℕ).  -/
 theorem Equation1_maximal (l : MagmaLaw ℕ) : l ≤ (0 ≃ 0) :=
-  fun _ _ ↦ rfl
+  fun _ _ _ _ ↦ rfl
 
 theorem Equation2_all_eq {G} [Magma G] (h : G ⊧ (0 ≃ 1 : MagmaLaw ℕ)) :
     ∀ (x y : G), x = y := by
@@ -48,7 +60,7 @@ theorem Equation2_all_eq {G} [Magma G] (h : G ⊧ (0 ≃ 1 : MagmaLaw ℕ)) :
     | 1 => y
     | _ => x)
 
-theorem Equation2_implies (l : MagmaLaw ℕ) : (0 ≃ 1).implies l := by
+theorem Equation2_implies (l : MagmaLaw ℕ) : (0 ≃ 1 : MagmaLaw ℕ).implies l := by
   intro G _ h φ
   have hG := Equation2_all_eq h
   simp only [satisfiesPhi]
@@ -81,5 +93,9 @@ theorem Law.implies_fin_implies_nat {n : Nat} {l₁ l₂ : MagmaLaw (Fin n)}
 theorem Law.leq_fin_leq_nat {n : Nat} {l₁ l₂ : MagmaLaw (Fin n)} (h : l₁ ≤ l₂) :
     l₁.map Fin.val ≤ l₂.map Fin.val :=
   implies_fin_implies_nat h
+
+theorem reindex_iff {α β} {Law1 : MagmaLaw α} {Law2 : MagmaLaw β} (f g)
+    (h1 : Law1.map f = Law2) (h2 : Law2.map g = Law1) : Law1.iff Law2 :=
+  fun _ _ => ⟨h1 ▸ satisfies_map _, h2 ▸ satisfies_map _⟩
 
 end Law.MagmaLaw
