equational_theories/Duals/Basic.lean
@@ -1,0 +1,26 @@
+import equational_theories.Equations.Basic
+import equational_theories.Duals.Command
+
+duals 1 ↔ 1
+duals 2 ↔ 2
+duals 3 ↔ 3
+duals 4 ↔ 5
+duals 6 ↔ 6
+duals 7 ↔ 7
+duals 8 ↔ 23
+duals 14 ↔ 29
+duals 38 ↔ 39
+duals 40 ↔ 40
+duals 41 ↔ 41
+duals 42 ↔ 45
+duals 43 ↔ 43
+duals 46 ↔ 46
+duals 168 ↔ 168
+duals 1485 ↔ 2162
+duals 3588 ↔ 3994
+duals 3722 ↔ 3722
+duals 3744 ↔ 3744
+duals 4512 ↔ 4512
+duals 4513 ↔ 4564
+duals 4522 ↔ 4579
+duals 4582 ↔ 4582
